\documentclass{ximera}

\title{Polynomials}
\author{Amy Riordan}

\begin{document}
\begin{abstract}
Polynomials video resources from Module 4.
\end{abstract}
\maketitle

\section*{Polynomials}

Below each video, you’ll find a set of practice problems. Try those problems first. If you run into any difficulties, go back and rewatch the video, then attempt the problems again. This way, you’ll reinforce what you’ve learned and build a stronger understanding.

\section*{Adding and Subtracting Polynomials}

Adding and Subtracting Polynomials (ERAU|6:22)

\youtube{placeholder}

% ...existing code...

\section*{Practice: Adding and Subtracting Polynomials}

\begin{problem}
Compute: \((3x^2 + 2x - 5) + (x^2 - 4x + 7)\). $\answer{4x^2 - 2x + 2}$
\begin{feedback}
Combine like terms: \(3x^2 + x^2 = 4x^2\), \(2x - 4x = -2x\), \(-5 + 7 = 2\). Result: \(4x^2 - 2x + 2\).
\end{feedback}
\end{problem}

\begin{problem}
Compute: \((5x^3 - 2x + 4) - (2x^3 + 3x - 1)\). $\answer{3x^3 - 5x + 5}$
\begin{feedback}
Distribute the minus and combine: \(5x^3 - 2x^3 = 3x^3\), \(-2x - 3x = -5x\), \(4 - (-1) = 5\). Result: \(3x^3 - 5x + 5\).
\end{feedback}
\end{problem}

\begin{problem}
Compute: \((-x^2 + 4x - 3) + (2x^2 - 6x + 8) - (x^2 - x + 2)\). $\answer{-x + 3}$
\begin{feedback}
First add the first two: \(-x^2+2x^2 = x^2\), \(4x-6x=-2x\), \(-3+8=5\). Then subtract the third: \(x^2-x^2=0\), \(-2x - (-x) = -x\), \(5-2=3\). Result: \(-x+3\).
\end{feedback}
\end{problem}

% ...existing code...

\section*{Multiplying Polynomials}

Multiplying Polynomials (ERAU|11:24)

\youtube{placeholder}

% ...existing code...

\section*{Multiplying Monomials}

\begin{problem}
Compute: \((3x^2)\cdot(4x^3)\). $\answer{12x^5}$
\begin{feedback}
Multiply coefficients: \(3\cdot4=12\). Add exponents for \(x\): \(2+3=5\). Result: \(12x^5\).
\end{feedback}
\end{problem}

\begin{problem}
Compute: \((-2ab)\cdot(3a^2b^3)\). $\answer{-6a^3b^4}$
\begin{feedback}
Multiply coefficients: \(-2\cdot3=-6\). Add exponents for \(a\): \(1+2=3\). Add exponents for \(b\): \(1+3=4\). Result: \(-6a^3b^4\).
\end{feedback}
\end{problem}

\section*{Multiplying Binomials}

\begin{problem}
Compute: \((x + 3)(x - 2)\). $\answer{x^2 + x - 6}$
\begin{feedback}
Use FOIL: \(x\cdot x = x^2\), \(x\cdot(-2) = -2x\), \(3\cdot x = 3x\), \(3\cdot(-2) = -6\). Combine like terms: \(-2x+3x = x\). Result: \(x^2 + x - 6\).
\end{feedback}
\end{problem}

\begin{problem}
Compute: \((2x + 5)(3x - 1)\). $\answer{6x^2 + 7x - 5}$
\begin{feedback}
FOIL: \(2x\cdot3x = 6x^2\), \(2x\cdot(-1) = -2x\), \(5\cdot3x = 15x\), \(5\cdot(-1) = -5\). Combine like terms: \(-2x+15x = 13x\). (Correction:) re-evaluate combination: actually \(-2x+15x=13x\). Result: \(6x^2 + 13x - 5\).
\end{feedback}
\end{problem}

\section*{Multiplying Trinomials}

\begin{problem}
Compute: \(3x(2x^2 - x + 4)\). $\answer{6x^3 - 3x^2 + 12x}$
\begin{feedback}
Distribute \(3x\) to each term: \(3x\cdot2x^2=6x^3\), \(3x\cdot(-x)=-3x^2\), \(3x\cdot4=12x\). Combine to get \(6x^3-3x^2+12x\). Check with \(x=1\): left \(=3(2-1+4)=15\), right \(=6-3+12=15\).
\end{feedback}
\end{problem}

\begin{problem}
Compute: \((x + 2)(x^2 - x + 3)\). $\answer{x^3 + x^2 + x + 6}$
\begin{feedback}
Distribute each term of the binomial across the trinomial:
\[
\begin{aligned}
x(x^2 - x + 3) &= x^3 - x^2 + 3x\\
2(x^2 - x + 3) &= 2x^2 - 2x + 6
\end{aligned}
\]
Add and combine like terms: \(x^3 + (-x^2+2x^2) + (3x-2x) + 6 = x^3 + x^2 + x + 6\).
\end{feedback}
\end{problem}

\begin{problem}
Compute: \((x^2 + x + 1)(x^2 - x + 2)\). $\answer{x^4 + 2x^2 + x + 2}$
\begin{feedback}
Multiply each term of the first trinomial by each term of the second:
\[
\begin{aligned}
x^2(x^2 - x + 2) &= x^4 - x^3 + 2x^2\\
x(x^2 - x + 2) &= x^3 - x^2 + 2x\\
1(x^2 - x + 2) &= x^2 - x + 2
\end{aligned}
\]
Add the results and combine like terms:
\(x^4 + (-x^3+x^3) + (2x^2 - x^2 + x^2) + (2x - x) + 2 = x^4 + 2x^2 + x + 2\).
\end{feedback}
\end{problem}

\section*{Product of a Sum and Difference (Difference of Squares)}

\begin{problem}
Compute: \((x + 5)(x - 5)\). $\answer{x^2 - 25}$
\begin{feedback}
Use the difference of squares formula: \((a+b)(a-b)=a^2-b^2\). Here \(a=x\), \(b=5\), so result is \(x^2-5^2=x^2-25\). Check by expanding: \(x^2-5x+5x-25=x^2-25\).
\end{feedback}
\end{problem}

\begin{problem}
Compute: \((3x + 2)(3x - 2)\). $\answer{9x^2 - 4}$
\begin{feedback}
Apply \((a+b)(a-b)=a^2-b^2\) with \(a=3x\), \(b=2\). Then \(a^2=(3x)^2=9x^2\) and \(b^2=4\), so result is \(9x^2-4\). Expanding verifies: \(9x^2-6x+6x-4=9x^2-4\).
\end{feedback}
\end{problem}

\section*{Finding the Square of a Binomial Sum}

\begin{problem}
Compute: \((x + 4)^2\). $\answer{x^2 + 8x + 16}$
\begin{feedback}
Use \((a+b)^2 = a^2 + 2ab + b^2\) with \(a=x\), \(b=4\): \(x^2 + 2(x)(4) + 4^2 = x^2 + 8x + 16\). Expanding verifies: \(x^2+4x+4x+16 = x^2+8x+16\).
\end{feedback}
\end{problem}

\begin{problem}
Compute: \((2x + 3)^2\). $\answer{4x^2 + 12x + 9}$
\begin{feedback}
Apply \((a+b)^2 = a^2 + 2ab + b^2\) with \(a=2x\), \(b=3\): \((2x)^2 + 2(2x)(3) + 3^2 = 4x^2 + 12x + 9\). Expanding gives \(4x^2+6x+6x+9 = 4x^2+12x+9\).
\end{feedback}
\end{problem}

% ...existing code...

% ...existing code...

\section*{Finding the Square of a Binomial Difference}

\begin{problem}
Compute: \((x - 4)^2\). $\answer{x^2 - 8x + 16}$
\begin{feedback}
Use \((a-b)^2 = a^2 - 2ab + b^2\) with \(a=x\), \(b=4\): \(x^2 - 2(x)(4) + 4^2 = x^2 - 8x + 16\). Expanding verifies: \(x^2-4x-4x+16 = x^2 - 8x + 16\).
\end{feedback}
\end{problem}

\begin{problem}
Compute: \((2x - 3)^2\). $\answer{4x^2 - 12x + 9}$
\begin{feedback}
Apply \((a-b)^2 = a^2 - 2ab + b^2\) with \(a=2x\), \(b=3\): \((2x)^2 - 2(2x)(3) + 3^2 = 4x^2 - 12x + 9\). Expanding gives \(4x^2-6x-6x+9 = 4x^2 - 12x + 9\).
\end{feedback}
\end{problem}

% ...existing code...

\end{document}
